rich_raven_lang/trnsl.v
@@ -25,18 +25,24 @@ Section MainTranslation.
       set_fold (λ inv acc, acc ∪ ↑(inv_namespace_map inv)) ∅ s.
 
     Lemma inv_map_subseteq invr mask:
-      invr ∈ mask -> ↑inv_namespace_map invr ⊆ inv_set_to_namespace mask.
+      invr ∈ mask -> ↑(inv_namespace_map invr) ⊆ inv_set_to_namespace mask.
     Proof.
-      Admitted.
+      revert mask.
+      unfold inv_set_to_namespace.
+      apply (set_fold_ind (λ acc s, invr ∈ s → ↑inv_namespace_map invr ⊆ acc)).
+    - solve_proper.
+    - intros Hcontra. set_solver.
+    - intros x s' acc Hnotin IH Hin'.
+      destruct (decide (x = invr)) as [->|Hneq].
+      + set_solver.
+      + set_solver.
+    Qed.
 
     Lemma inv_map_set_minus_subseteq mask invr:
       invr ∈ mask ->
         (inv_set_to_namespace (mask ∖ {[invr]})) = inv_set_to_namespace mask ∖ ↑inv_namespace_map invr.
     Proof.
       Admitted.
-
-    (* Definition symb_stk_to_stk_frm (stk : stack) (mp : symb_map) : stack_frame :=
-      StackFrame (fmap (λ v, trnsl_lval (mp v)) stk). *)
 
     Lemma trnsl_expr_interp_lexpr_compatibility stk e lexpr lv mp : 
       trnsl_expr_lExpr stk e = Some (lexpr) -> 
@@ -50,22 +56,20 @@ Section MainTranslation.
       interp_lexpr lexpr mp = Some lv.
     Admitted.
 
-    Definition trnsl_hoare_triple Γ (stk_id: stack_id) (p : assertion) (ι1: nat) (msk : maskAnnot) (cmd : stmt) (q : assertion) (ι2: nat) (mp : symb_map) : iProp rrl_lang.Σ :=
+    Definition trnsl_hoare_triple (stk_id: stack_id) (p : assertion) (ι1: nat) (msk : maskAnnot) (cmd : stmt) (q : assertion) (ι2: nat) (mp : symb_map) : iProp rrl_lang.Σ :=
         match (trnsl_stmt cmd) with 
         | Error => True
         | None' =>
-          match (trnsl_assertion Γ p stk_id mp), 
-                (trnsl_assertion Γ q stk_id mp) with
-          | None, _ | _, None => True
-          | Some p', Some q' =>
+          match (trnsl_assertion p stk_id mp), 
+                (trnsl_assertion q stk_id mp) with
+          | p', q' =>
             p' ∗ £ ι1 ={inv_set_to_namespace msk}=∗ q' ∗ £ ι2 
           end
         
         | Some' s =>
-          match (trnsl_assertion Γ p stk_id mp), 
-                (trnsl_assertion Γ q stk_id mp) with
-          | None, _ | _, None => True
-          | Some p', Some q' => 
+          match (trnsl_assertion p stk_id mp), 
+                (trnsl_assertion q stk_id mp) with
+          | p', q' => 
             {{{ p' ∗ £ ι1 }}}  
               to_rtstmt stk_id s @ (inv_set_to_namespace msk)
             {{{ RET lang.LitUnit; q' ∗ £ ι2}}}
@@ -180,7 +184,7 @@ Section MainTranslation.
     Qed.
 
     Axiom proc_specs_valid :
-      forall Γ proc proc_record stk_vals, 
+      forall proc proc_record stk_vals, 
       proc ∈ proc_set  ->
       proc_map !! proc = Some proc_record ->
 
@@ -193,8 +197,8 @@ Section MainTranslation.
 
       let subst_map' := list_to_map (zip (proc_args_of proc_record).*1 (map (λ val, LVal (trnsl_val val)) stk_vals)) in
 
-      trnsl_assertion Γ (subst (proc_precond_of proc_record) subst_map') stk_id mp = Some precond ->
-      trnsl_assertion Γ (subst (proc_postcond_of proc_record) (<["#ret_val" := LVal (trnsl_val (ret_val))]> subst_map')) stk_id mp = Some postcond ->
+      trnsl_assertion (subst (proc_precond_of proc_record) subst_map') stk_id mp = precond ->
+      trnsl_assertion (subst (proc_postcond_of proc_record) (<["#ret_val" := LVal (trnsl_val (ret_val))]> subst_map')) stk_id mp = postcond ->
       
       ((trnsl_stmt (proc_body_of proc_record) = Some' stmt) \/ (trnsl_stmt (proc_body_of proc_record) = None' /\ stmt = lang.SkipS) ) ->
       (∃ stk_frm'',
@@ -206,11 +210,11 @@ Section MainTranslation.
       unfold transport. revert Hupd.
     (* usually trivial by proper instance or f_equiv *) Admitted. *)
 
-    Theorem rrl_validity Γ ρ σ ι1 ι2 stk_id p msk cmd q :
+    Theorem rrl_validity ρ σ ι1 ι2 stk_id p msk cmd q :
       stmt_well_defined ρ cmd -> 
       forall mp, (env_typ_well_defined σ mp) ->
        ⌜RavenHoareTriple ρ σ p ι1 cmd msk q ι2⌝
-      ⊢  (trnsl_hoare_triple Γ stk_id p ι1 msk cmd q ι2 mp).
+      ⊢  (trnsl_hoare_triple stk_id p ι1 msk cmd q ι2 mp).
     Proof.
       iIntros (Hwelldef mp Henv) "%H". 
       iInduction H as 
@@ -228,8 +232,9 @@ Section MainTranslation.
 
         inversion Ht. simpl. 
         - iIntros (Φ). iModIntro.
+          setoid_rewrite trnsl_assertion_unfold.
           iIntros "[[Hstk1 Hstk2] Hcred] HΦ".
-
+          simpl.
           iDestruct "Hstk2" as "[%l [%Hlexpr1 Hlfld]]".
           
           iApply (wp_heap_wr stk_id (symb_stk_to_stk_frm stk mp) _ _ _ l _ _ _ with "[Hstk1 Hlfld]").
@@ -264,37 +269,32 @@ Section MainTranslation.
         (* INV ACCESS BLOCK *)
         unfold trnsl_hoare_triple.
 
-        pose proof (trnsl_inv_validity Γ invr lexprs stk_id mp) as Htrnsl_inv_valid.
+        pose proof (trnsl_inv_validity' invr lexprs stk_id mp) as Htrnsl_inv_valid.
         rewrite Hinv_record in Htrnsl_inv_valid. simpl in Htrnsl_inv_valid.
-        destruct (trnsl_assertion Γ (rrl_lang.subst (inv_body inv_record)
-        subst) stk_id mp) eqn:HinvBody. 2:{ rewrite HinvBody in Htrnsl_inv_valid. inversion Htrnsl_inv_valid. }
-
-        rewrite HinvBody in Htrnsl_inv_valid. injection Htrnsl_inv_valid as Htrnsl_inv.
         
         destruct (trnsl_stmt (InvAccessBlock invr args stmt)) eqn:Ht. 
         2: { done. }
 
         
         { 
-          destruct (trnsl_assertion Γ (LStack stk) stk_id mp) eqn:Hstack.
-          2 : { simpl in Hstack. inversion Hstack. }
+          destruct (trnsl_assertion (LStack stk) stk_id mp) eqn:Hstack.
 
-          simpl. rewrite HinvBody. 
-           destruct (trnsl_assertion Γ p stk_id mp) eqn:Hp, (trnsl_assertion Γ q stk_id mp) eqn:Hq; try done.
+          simpl.
+          setoid_rewrite trnsl_assertion_unfold. simpl.
+          iIntros "[Hpre Hcr]".
+          iDestruct "Hpre" as "[Hstk Hrest]".
+          rewrite Hinv_record.
+          iDestruct "Hrest" as "[#H Hu]".
            
-           iIntros "[[Hstk [#H Hu]] Hcr]".
-           (* unfold trnsl_hoare_triple in IH. *)
            assert (trnsl_stmt stmt = None'). {
             apply trnsl_stmt_trnsl_atomic_block_none. simpl in Ht. exact Ht. }
            iEval (rewrite H) in "IH".
-           (* rewrite Hp Hq in IHHbody. *)
 
           iInv "H" as "Hinv".
           { 
             (* inv_namespace mask *)
             apply inv_map_subseteq; try done.
           }
-          rewrite <- Htrnsl_inv.
 
           assert (ι1 = (ι1-1 + 1)) as Hiota. { rewrite Nat.sub_add; [ reflexivity | ]. lia. }
           apply (f_equal lc) in Hiota.
@@ -309,34 +309,31 @@ Section MainTranslation.
           
           
           iPoseProof ("IH" with  "[%] [%] [Hcomb Hcr1]") as "IH2"; try iFrame; try done.
+          { setoid_rewrite trnsl_assertion_unfold. iFrame.  }
           assert ((inv_set_to_namespace (mask ∖ {[invr]})) = inv_set_to_namespace mask ∖ ↑inv_namespace_map invr) as HInvs. { apply inv_map_set_minus_subseteq; try done. }
           rewrite HInvs.
           iDestruct "IH2" as ">IH2".
+          setoid_rewrite trnsl_assertion_unfold.
           iDestruct "IH2" as "[[IHs [IHH1 IHH] ] Hcr]".
           iModIntro.
           iFrame "# ∗". done.
-
-          (* pose proof (trnsl_inv_validity invr lexprs mp) as Htrnsl_inv_valid. *)
         }
         
         { 
           assert (trnsl_stmt stmt = Some' s). {
             apply trnsl_stmt_trnsl_atomic_block_some. simpl in Ht. exact Ht. }
           simpl.
-          iEval (rewrite H HinvBody) in "IH" .
-          (* iEval (rewrite Hinv_record). *)
-          destruct (trnsl_assertion Γ p stk_id mp) eqn:Hp, (trnsl_assertion Γ q stk_id mp) eqn:Hq; try done.
           iIntros (Φ).
           iModIntro.
+          setoid_rewrite trnsl_assertion_unfold.
           iIntros "[[Hstk [#HInv Hu]] Hcr] HΦ".
-          rewrite <- Htrnsl_inv.
 
           assert (ι1 = (ι1-1 + 1)) as Hiota. { rewrite Nat.sub_add; [ reflexivity | ]. lia. }
           apply (f_equal lc) in Hiota.
           iEval (rewrite Hiota) in "Hcr".
 
           iPoseProof ((lc_split (ι1 - 1) 1) with "Hcr") as "[Hcr1 Hcr2]".
-
+          rewrite Hinv_record.
           iInv "HInv" as "HInvBody".
           { 
             (* inv_namespace mask *)
@@ -358,13 +355,18 @@ Section MainTranslation.
           rewrite H0; destruct H0.
 
           inversion Hwelldef as [ | | | | | | | | | | | | | inv args' stmt' HInvSet HargsWellDef HBodywelldef | ]; subst stmt' args'.
+          iEval (rewrite H) in "IH".
           iApply ("IH" with "[%] [%] [Hcomb Hcr1]"); try iFrame; try done.
+          { rewrite Htrnsl_inv_valid. setoid_rewrite trnsl_assertion_unfold. iFrame. }
           iNext.
+          setoid_rewrite trnsl_assertion_unfold.
           iIntros "[[Hstk [Hu Hu1]] Hcr]".
           iModIntro.
           iFrame.
           iApply "HΦ".
           iFrame "# ∗".
+          rewrite Hinv_record.
+          setoid_rewrite trnsl_assertion_unfold. iExact "HInv".
         }
       }
 
@@ -381,6 +383,7 @@ Section MainTranslation.
         { iApply (wp_assign stk_id (symb_stk_to_stk_frm stk mp) v (trnsl_lval v0) e with "[Hstk]").
 
           {
+            setoid_rewrite trnsl_assertion_unfold.
             iFrame.
             iPureIntro.
             apply (trnsl_expr_interp_lexpr_compatibility _ _ lexpr). { done. } 
@@ -391,6 +394,7 @@ Section MainTranslation.
           iIntros "[Hstk Hcr1]".
           iApply "HΦ".
           iCombine "Hcr" "Hcr1" as "Hcr". rewrite Nat.add_1_r. iFrame.
+          setoid_rewrite trnsl_assertion_unfold.
           iExists (v0).
           iSplitL.
           {
@@ -438,19 +442,16 @@ Section MainTranslation.
         unfold trnsl_hoare_triple. simpl.
         destruct (trnsl_stmt s) eqn:Htrnsl; try done.
         { simpl.
-          destruct (trnsl_assertion Γ p stk_id mp) eqn:Hp, (trnsl_assertion Γ q stk_id mp) eqn:Hq, (trnsl_assertion Γ r stk_id mp) eqn:Hr; try done. 
+          setoid_rewrite trnsl_assertion_unfold.
 
           iIntros "[[Hu Hu1] Hcr]".
           iPoseProof ("IH2" with "[%] [Hu Hcr]") as ">[IH3 Hcr']"; try iFrame; try done.
 
         }
 
-        { 
-          destruct (trnsl_assertion Γ p stk_id mp) eqn:Hp, 
-                   (trnsl_assertion Γ q stk_id mp) eqn:Hq, 
-                   (trnsl_assertion Γ r stk_id mp) eqn:Hr; try done.
-
+        {
           iIntros (Φ).
+          setoid_rewrite trnsl_assertion_unfold.
           iModIntro. iIntros "[[Hu Hu1] Hcr] HΦ".
           iApply ("IH2" with "[%] [Hu Hcr]"); try iFrame; try done.
           iNext. iIntros "[Hu0 Hcr']". iApply "HΦ". iFrame.
@@ -460,7 +461,7 @@ Section MainTranslation.
       1 : {
         (* FIELD READ *)
         unfold trnsl_hoare_triple; simpl.
-        iIntros (Φ). iModIntro. iIntros "[[Hstk Hl] Hcr] HΦ".
+        iIntros (Φ). setoid_rewrite trnsl_assertion_unfold. iModIntro. iIntros "[[Hstk Hl] Hcr] HΦ".
         iDestruct "Hl" as (l) "[%HLe_h H_l_hp]".
 
         destruct (interp_lexpr lexpr_e mp) eqn: Hinterp.
@@ -510,11 +511,13 @@ Section MainTranslation.
         iModIntro.
         iIntros "[Hstack Hcr] HΦ".
         iApply (wp_alloc with "[Hstack]") .
-        - iFrame.
+        - done.
+        - setoid_rewrite trnsl_assertion_unfold. iFrame.
         - iNext.
           iIntros "Hpost".
           iDestruct "Hpost" as (l) "[Hstk [Hhp Hcr']]".
           iApply "HΦ". iCombine "Hcr" "Hcr'" as "Hcr". rewrite Nat.add_1_r. iFrame.
+          setoid_rewrite trnsl_assertion_unfold.
           iExists (LitLoc l).
           set (mp' := (λ x0 : lvar, if (x0 =? lvar_x)%string then LitLoc l else mp x0)).
 
@@ -522,44 +525,50 @@ Section MainTranslation.
           
           + simpl. iFrame. rewrite fresh_mp_rewrite_symb_stk_to_stk_frm_compat; try done.
           unfold symb_stk_to_stk_frm. simpl. 
-          assert (lang.LitLoc l = lang.LitLoc {| loc_car := loc_car l |}) as H1.
+          assert (lang.LitLoc l = lang.LitLoc {| loc_car := loc_car l |}) as H1'.
           {  destruct l. simpl. done. }
-          rewrite <- H1. iFrame.
+          rewrite <- H1'. iFrame.
 
           + simpl. destruct a as [fld val].
           assert (stmt_well_defined ρ (Alloc x fld_vals)) as Hwell_def'. { apply (alloc_stmt_well_defined _ _ fld val). exact Hwelldef. }
-          destruct (trnsl_assertion Γ (field_list_to_assertion (LVar lvar_x) fld_vals) stk_id mp' ) eqn:Htrfl.
           
-            * simpl. rewrite Htrfl.
+            * simpl. 
               iPoseProof ("IH" with "[%]") as "IH2"; try done.
               iClear "IH".
               iDestruct "Hhp" as "[Hhpl Hhpfvs]".
-              iPoseProof ("IH2" with "Hstk Hhpfvs") as "[IH3 IH3']". 
+              inversion H0.
+              iPoseProof ("IH2" $! H5 with "Hstk Hhpfvs") as "[IH3 IH3']". 
               iFrame. iExists l. 
-              assert (trnsl_lval (trnsl_val val) = val) as H1. { apply trnsl_lval_trnsl_val_inverse. } 
-              rewrite H1. iFrame.
+              assert (trnsl_lval (trnsl_val val) = val) as H1'. { apply trnsl_lval_trnsl_val_inverse. } 
+              rewrite H1'. iFrame.
               iPureIntro. 
               unfold LExpr_holds.
               simpl.
               subst mp'. simpl. rewrite String.eqb_refl. rewrite val_beq_refl. done.
-
-            * simpl. rewrite Htrfl. iPoseProof ("IH" with "[%]") as "IH2"; try done.
       }
 
       4 : {
         (* UNFOLD PRED *)
         unfold trnsl_hoare_triple.
         simpl.
-        pose proof (trnsl_pred_validity Γ pred lexprs stk_id mp) as HPredTrnsl. rewrite H0 in HPredTrnsl. unfold subst_map in HPredTrnsl. rewrite HPredTrnsl.
-        iIntros. iModIntro.  iFrame.
+        pose proof (trnsl_pred_validity' pred lexprs stk_id mp) as HPredTrnsl. rewrite H0 in HPredTrnsl. unfold subst_map in HPredTrnsl. setoid_rewrite trnsl_assertion_unfold in HPredTrnsl. 
+        setoid_rewrite trnsl_assertion_unfold.
+        simpl.
+        rewrite <- HPredTrnsl.
+        iIntros "[[Hstk Hpred] Hcr]".
+        iPoseProof ((lc_split ι 1) with "Hcr") as "[Hcr1 Hcr2]".
+
+        iDestruct (lc_fupd_elim_later with "Hcr2 Hpred") as ">Hpred".
+        iFrame. done.
+
       }
 
       4 : {
         (* FOLD PRED *)
         unfold trnsl_hoare_triple.
         simpl.
-        pose proof (trnsl_pred_validity Γ pred lexprs stk_id mp) as HPredTrnsl. rewrite H1 in HPredTrnsl. unfold subst_map in HPredTrnsl. rewrite HPredTrnsl.
-        iIntros. iModIntro.  iFrame.
+        pose proof (trnsl_pred_validity' pred lexprs stk_id mp) as HPredTrnsl. rewrite H1 in HPredTrnsl. unfold subst_map in HPredTrnsl. setoid_rewrite trnsl_assertion_unfold. simpl. rewrite H1. rewrite HPredTrnsl.
+        iIntros "[[Hstk HPred] Hcr]". iModIntro. rewrite <- HPredTrnsl. iFrame. iNext. setoid_rewrite trnsl_assertion_unfold. iFrame.
       }
 
       2 : {
@@ -571,53 +580,40 @@ Section MainTranslation.
 
         unfold trnsl_hoare_triple. 
         simpl.
-        destruct (trnsl_assertion Γ a2 stk_id mp) eqn:Ha2.
         - destruct (trnsl_stmt c1) eqn:Hc1, (trnsl_stmt c2) eqn:Hc2; try done.
-          + destruct (trnsl_assertion Γ a1 stk_id mp) eqn:Ha1, (trnsl_assertion Γ a3 stk_id mp) eqn: Ha3; try done. iIntros "Hu0".
+          +  iIntros "Hu0".
           iPoseProof ("IH'" with "[%] Hu0") as ">IHH"; try done.
            iApply "IH1'"; try done.
 
-          + destruct (trnsl_assertion Γ a1 stk_id mp) eqn:Ha1, (trnsl_assertion Γ a3 stk_id mp) eqn: Ha3; try done. 
-            iIntros (Φ). iModIntro. iIntros "Hu0 HΦ".
+          + iIntros (Φ). iModIntro. iIntros "Hu0 HΦ".
             iPoseProof ("IH'" with "[%] Hu0") as ">IHH"; try done.
             iApply ("IH1'" with "[%] IHH"); try done.
 
-          + destruct (trnsl_assertion Γ a1 stk_id mp) eqn:Ha1, (trnsl_assertion Γ a3 stk_id mp) eqn: Ha3; try done.
-
-            iIntros (Φ) "!> [Hu0 Hcr] HΦ".
+          + iIntros (Φ) "!> [Hu0 Hcr] HΦ".
             iApply wp_fupd.
             iApply ("IH'" $! Henv with "[$Hu0 $Hcr]").
             iNext. iIntros "Hmid".
             iPoseProof ("IH1'" $! Henv with "Hmid") as "Hpost".
             iMod "Hpost". iModIntro. iApply "HΦ". iFrame.
 
-          + destruct (trnsl_assertion Γ a1 stk_id mp) eqn:Ha1, (trnsl_assertion Γ a3 stk_id mp) eqn: Ha3; try done.
-          simpl.
-          iApply wp_seq.
-            { iApply "IH'"; try done. }
-            { iApply "IH1'"; try done. }
-
-        (* Case: trnsl_assertion a2 = None; *)
-        - assert (is_Some (trnsl_assertion Γ a2 stk_id mp )) as Hassert. 
-          { apply trnsl_assertion_is_some. }
-          destruct Hassert. rewrite H6 in Ha2. discriminate.
-
-           
+          + simpl.
+            iApply wp_seq.
+              { iApply "IH'"; try done. }
+              { iApply "IH1'"; try done. }
       }
 
       5 : {
         (* SKIP *)
         unfold trnsl_hoare_triple. simpl.
-        destruct (trnsl_assertion Γ p stk_id mp); try done.
         iIntros (Φ). iModIntro. iIntros "[Hp Hcr] HΦ".
         iApply (wp_skip with "Hp"). 
-        iNext. iIntros "[[Hstk Hu] Hcr']". iApply "HΦ". iCombine "Hcr" "Hcr'" as "Hcr". iFrame.
+        iNext. setoid_rewrite trnsl_assertion_unfold. iIntros "[[Hstk Hu] Hcr']". iApply "HΦ". iCombine "Hcr" "Hcr'" as "Hcr". iFrame.
       }
 
       5: {
         (* CAS SUCC *)
         unfold trnsl_hoare_triple; simpl.
-        iIntros (Φ). iModIntro. iIntros "[[Hstk He1] Hcr] HΦ".
+        iIntros (Φ). iModIntro. setoid_rewrite trnsl_assertion_unfold. iIntros "[[Hstk He1] Hcr] HΦ".
         iDestruct "He1" as (l) "[%He1 Hl]".
         assert (interp_lexpr (LVal old_val) mp = Some old_val) as Hinterp_old; try done.
         assert (interp_lexpr (LVal new_val) mp = Some new_val) as Hinterp_new; try done.
@@ -669,7 +665,7 @@ Section MainTranslation.
       5 : {
         (* CAS FAIL *)
         unfold trnsl_hoare_triple; simpl.
-        iIntros (Φ). iModIntro. iIntros "[[Hstk [He1 %Hneq]] Hcr] HΦ".
+        iIntros (Φ). iModIntro. setoid_rewrite trnsl_assertion_unfold. iIntros "[[Hstk [He1 %Hneq]] Hcr] HΦ".
         iDestruct "He1" as (l) "[%He1 Hl]".
         assert (interp_lexpr (LVal old_val2) mp = Some old_val2) as Hinterp_old; try done.
         pose proof (trnsl_expr_interp_lexpr_compatibility _ _ _ _ _ H2 Hinterp_old) as Hexpr_step_e2.
@@ -733,10 +729,10 @@ Section MainTranslation.
         (* WEAKENING *)
         unfold entails in *.
         unfold trnsl_hoare_triple. simpl.
-        specialize H0 with Γ stk_id mp.
+        specialize H0 with stk_id mp.
         destruct H0 as [P' [P [HP' [HP HP_ent_P']]]].
         
-        specialize H1 with Γ stk_id mp.
+        specialize H1 with stk_id mp.
         destruct H1 as [Q [Q' [HQ [HQ' HQ_ent_Q']]]].
         rewrite HP HP' HQ HQ'.
 
@@ -774,12 +770,11 @@ Section MainTranslation.
           unfold typeOf in Hle_typ. destruct (trnsl_lval val0) eqn:Hle_val; try done.
           unfold trnsl_lval in Hle_val. destruct (val0) eqn: Hle_val'; try done.
 
-        destruct (trnsl_stmt s1) eqn:Hs1, (trnsl_stmt s2) eqn:Hs2; try done;
-        destruct (trnsl_assertion Γ p stk_id mp) eqn:HP, (trnsl_assertion Γ q stk_id mp) eqn:HQ; try done.
+        destruct (trnsl_stmt s1) eqn:Hs1, (trnsl_stmt s2) eqn:Hs2; try done.
 
         - destruct b0.
 
-          + iIntros "[[Hstk Hu] Hcr]".
+          + setoid_rewrite trnsl_assertion_unfold. iIntros "[[Hstk Hu] Hcr]".
 
           iPoseProof ("IH'" with "[%] [Hstk Hu Hcr]") as "Hpost"; try iFrame; try done.
           { unfold LExpr_holds. rewrite Hinterp_lexpr. done. }
@@ -794,7 +789,7 @@ Section MainTranslation.
 
           iFrame. iModIntro. done.
           
-          + iIntros "[[Hstk Hu] Hcr]".
+          + setoid_rewrite trnsl_assertion_unfold. iIntros "[[Hstk Hu] Hcr]".
 
           iPoseProof ("IH1'" with "[%] [Hstk Hu Hcr]") as "Hpost"; try iFrame; try done.
           { unfold LExpr_holds. simpl.  rewrite Hinterp_lexpr. done. }
@@ -809,16 +804,21 @@ Section MainTranslation.
           iFrame.
           done.
 
-        - iIntros (Φ). iModIntro. iIntros "[[Hstk Hu] Hcr] HΦ".
+        - iIntros (Φ). iModIntro. setoid_rewrite trnsl_assertion_unfold. iIntros "[[Hstk Hu] Hcr] HΦ".
           destruct b0.
-          + iApply (wp_if_t e (RTSkipS stk_id) (to_rtstmt stk_id s) stk_id (symb_stk_to_stk_frm stk1 mp) (u ∗ £ι1) (stack_own[ stk_id, symb_stk_to_stk_frm stk2 mp] ∗ u0 ∗ £ι2) (lang.LitUnit) (inv_set_to_namespace mask) with "[IH'] [IH' Hstk Hu Hcr] [HΦ]"); try iFrame.
+          + iApply (wp_if_t e (RTSkipS stk_id) (to_rtstmt stk_id s) stk_id (symb_stk_to_stk_frm stk1 mp) ((trnsl_assertion p stk_id mp) ∗ £ι1) (stack_own[ stk_id, symb_stk_to_stk_frm stk2 mp] ∗ (trnsl_assertion q stk_id mp) ∗ £ι2) (lang.LitUnit) (inv_set_to_namespace mask) with "[IH'] [IH' Hstk Hu Hcr] [HΦ]"); try iFrame.
             *  apply (trnsl_expr_interp_lexpr_compatibility _ e lexpr (LitBool true) mp); try done.
 
             * iIntros (Φ'). iModIntro. iIntros "[Hstk [Hu Hcr]] HΦ'".
+            setoid_rewrite trnsl_assertion_unfold.
             iPoseProof ("IH'" with "[%] [Hstk Hu Hcr]" ) as "HQ"; try done; try iFrame.
             { iPureIntro. unfold LExpr_holds. rewrite Hinterp_lexpr. done.  }
-            iDestruct "HQ" as ">[[Hstk Hu] Hcr]". iApply (wp_skip (stack_own[ stk_id, symb_stk_to_stk_frm stk2 mp] ∗ u0) with "[Hstk Hu]"); iFrame.
-            iNext. iIntros "[[Hstk Hu] Hcr']". iApply "HΦ'". iFrame. 
+            simpl.
+            iDestruct "HQ" as ">[[Hstk Hu] Hcr]". iApply (wp_skip (stack_own[ stk_id, symb_stk_to_stk_frm stk2 mp] ∗ (trnsl_assertion q stk_id mp)) with "[Hstk Hu]"); iFrame.
+            { setoid_rewrite trnsl_assertion_unfold. iFrame. }
+            iNext. iIntros "[[Hstk Hu] Hcr']". iApply "HΦ'". setoid_rewrite trnsl_assertion_unfold. iFrame.
+            
+            * setoid_rewrite trnsl_assertion_unfold. iFrame.
 
 
             * iNext. iIntros "[Hstk [Hu Hcr]]". iApply "HΦ". iFrame.
@@ -826,87 +826,103 @@ Section MainTranslation.
             assert (ι2 = ι2 `min` ι3 + (ι2 - ι2 `min` ι3)) as Hiota. { lia.  }
             apply (f_equal lc) in Hiota.
             iEval (rewrite Hiota) in "Hcr".
-            iDestruct (lc_split (ι2 `min` ι3) (ι2 - (ι2 `min` ι3)) with "Hcr") as "[Hcr2 Hcr2']". iFrame.
+            iDestruct (lc_split (ι2 `min` ι3) (ι2 - (ι2 `min` ι3)) with "Hcr") as "[Hcr2 Hcr2']". setoid_rewrite trnsl_assertion_unfold. iFrame.
           
-          + iApply (wp_if_f e (RTSkipS stk_id) (to_rtstmt stk_id s) stk_id (symb_stk_to_stk_frm stk1 mp) (u ∗ £ι1) (stack_own[ stk_id, symb_stk_to_stk_frm stk2 mp] ∗ u0 ∗ £ι3) (lang.LitUnit) (inv_set_to_namespace mask) with "[IH'] [IH' Hstk Hu Hcr] [HΦ]"); try iFrame.
+          + iApply (wp_if_f e (RTSkipS stk_id) (to_rtstmt stk_id s) stk_id (symb_stk_to_stk_frm stk1 mp) ((trnsl_assertion p stk_id mp) ∗ £ι1) (stack_own[ stk_id, symb_stk_to_stk_frm stk2 mp] ∗ (trnsl_assertion q stk_id mp) ∗ £ι3) (lang.LitUnit) (inv_set_to_namespace mask) with "[IH'] [IH' Hstk Hu Hcr] [HΦ]"); try iFrame.
             * apply (trnsl_expr_interp_lexpr_compatibility _ e lexpr (LitBool false) mp); try done.
 
             * iIntros (Φ'). iModIntro. iIntros "[Hstk [Hu Hcr]] HΦ'".
+            setoid_rewrite trnsl_assertion_unfold.
             iPoseProof ("IH1'" with "[%] [Hstk Hu Hcr]" ) as "HQ"; try done; try iFrame.
             { iPureIntro. unfold LExpr_holds. simpl. rewrite Hinterp_lexpr. done.  }
             iApply "HQ"; iFrame. iNext.
             iIntros "[[Hstk Hu] Hcr]". iApply "HΦ'". iFrame.
 
+            * setoid_rewrite trnsl_assertion_unfold. iFrame.
+
             * iNext. iIntros "[Hstk [Hu Hcr]]". iApply "HΦ". iFrame.
 
-            assert (ι3 = ι2 `min` ι3 + (ι3 - ι2 `min` ι3)) as Hiota. { lia.  }
+            assert (ι3 = ι2 `min` ι3 + (ι3 - ι2 `min` ι3)) as Hiota. { lia. }
             apply (f_equal lc) in Hiota.
             iEval (rewrite Hiota) in "Hcr".
-            iDestruct (lc_split (ι2 `min` ι3) (ι3 - (ι2 `min` ι3)) with "Hcr") as "[Hcr2 Hcr2']". iFrame.
+            iDestruct (lc_split (ι2 `min` ι3) (ι3 - (ι2 `min` ι3)) with "Hcr") as "[Hcr2 Hcr2']". setoid_rewrite trnsl_assertion_unfold. iFrame.
 
-        - iIntros (Φ). iModIntro. iIntros "[[Hstk Hu] Hcr] HΦ".
+        - iIntros (Φ). iModIntro. setoid_rewrite trnsl_assertion_unfold. iIntros "[[Hstk Hu] Hcr] HΦ".
           destruct b0.
-          + iApply (wp_if_t e (to_rtstmt stk_id s) (RTSkipS stk_id) stk_id (symb_stk_to_stk_frm stk1 mp) (u ∗ £ι1) (stack_own[ stk_id, symb_stk_to_stk_frm stk2 mp] ∗ u0 ∗ £ι2) (lang.LitUnit) (inv_set_to_namespace mask) with "[IH'] [IH' Hstk Hu Hcr] [HΦ]"); try iFrame.
+          + iApply (wp_if_t e (to_rtstmt stk_id s) (RTSkipS stk_id) stk_id (symb_stk_to_stk_frm stk1 mp) ((trnsl_assertion p stk_id mp) ∗ £ι1) (stack_own[ stk_id, symb_stk_to_stk_frm stk2 mp] ∗ (trnsl_assertion q stk_id mp) ∗ £ι2) (lang.LitUnit) (inv_set_to_namespace mask) with "[IH'] [IH' Hstk Hu Hcr] [HΦ]"); try iFrame.
             *  apply (trnsl_expr_interp_lexpr_compatibility _ e lexpr (LitBool true) mp); try done.
 
             * iIntros (Φ'). iModIntro. iIntros "[Hstk [Hu Hcr]] HΦ'".
+            setoid_rewrite trnsl_assertion_unfold.
             iPoseProof ("IH'" with "[%] [Hstk Hu Hcr]" ) as "HQ"; try done; try iFrame.
             { iPureIntro. unfold LExpr_holds. rewrite Hinterp_lexpr. done.  }
             iApply "HQ"; iFrame. iNext. iIntros "[[Hstk Hu] Hcr]". iApply "HΦ'". iFrame.
 
+            * setoid_rewrite trnsl_assertion_unfold. iFrame.
+
             * iNext. iIntros "[Hstk [Hu Hcr]]". iApply "HΦ". iFrame.
-            assert (ι2 = ι2 `min` ι3 + (ι2 - ι2 `min` ι3)) as Hiota. { lia.  }
+            assert (ι2 = ι2 `min` ι3 + (ι2 - ι2 `min` ι3)) as Hiota. { lia. }
             apply (f_equal lc) in Hiota.
             iEval (rewrite Hiota) in "Hcr".
-            iDestruct (lc_split (ι2 `min` ι3) (ι2 - (ι2 `min` ι3)) with "Hcr") as "[Hcr2 Hcr2']". iFrame.
+            iDestruct (lc_split (ι2 `min` ι3) (ι2 - (ι2 `min` ι3)) with "Hcr") as "[Hcr2 Hcr2']". setoid_rewrite trnsl_assertion_unfold. iFrame.
 
           
-          + iApply (wp_if_f e (to_rtstmt stk_id s) (RTSkipS stk_id) stk_id (symb_stk_to_stk_frm stk1 mp) (u ∗ £ι1) (stack_own[ stk_id, symb_stk_to_stk_frm stk2 mp] ∗ u0 ∗ £ι3) (lang.LitUnit) (inv_set_to_namespace mask) with "[IH'] [IH' Hstk Hu Hcr] [HΦ]"); try iFrame.
+          + iApply (wp_if_f e (to_rtstmt stk_id s) (RTSkipS stk_id) stk_id (symb_stk_to_stk_frm stk1 mp) ((trnsl_assertion p stk_id mp) ∗ £ι1) (stack_own[ stk_id, symb_stk_to_stk_frm stk2 mp] ∗ (trnsl_assertion q stk_id mp) ∗ £ι3) (lang.LitUnit) (inv_set_to_namespace mask) with "[IH'] [IH' Hstk Hu Hcr] [HΦ]"); try iFrame.
             * apply (trnsl_expr_interp_lexpr_compatibility _ e lexpr (LitBool false) mp); try done.
 
             * iIntros (Φ'). iModIntro. iIntros "[Hstk [Hu Hcr]] HΦ'".
+            setoid_rewrite trnsl_assertion_unfold.
             iPoseProof ("IH1'" with "[%] [Hstk Hu Hcr]" ) as "HQ"; try done; try iFrame.
-            { iPureIntro. unfold LExpr_holds. simpl. rewrite Hinterp_lexpr. done.  }
-            iDestruct "HQ" as ">[[Hstk Hu] Hcr]". iApply (wp_skip (stack_own[ stk_id, symb_stk_to_stk_frm stk2 mp] ∗ u0) with "[Hstk Hu]"); iFrame.
-            iNext. iIntros "[[Hstk Hu] Hcr']". iApply "HΦ'". iFrame.
+            { iPureIntro. unfold LExpr_holds. simpl. rewrite Hinterp_lexpr. done. }
+            
+            iDestruct "HQ" as ">[[Hstk Hu] Hcr]". iApply (wp_skip (stack_own[ stk_id, symb_stk_to_stk_frm stk2 mp] ∗ (trnsl_assertion q stk_id mp)) with "[Hstk Hu]"); iFrame.
+            { setoid_rewrite trnsl_assertion_unfold. iFrame. }
+            iNext. iIntros "[[Hstk Hu] Hcr']". iApply "HΦ'". setoid_rewrite trnsl_assertion_unfold. iFrame.
 
+            * setoid_rewrite trnsl_assertion_unfold. iFrame.
             * iNext. iIntros "[Hstk [Hu Hcr]]". iApply "HΦ". iFrame.
             
-            assert (ι3 = ι2 `min` ι3 + (ι3 - ι2 `min` ι3)) as Hiota. { lia.  }
+            assert (ι3 = ι2 `min` ι3 + (ι3 - ι2 `min` ι3)) as Hiota. { lia. }
             apply (f_equal lc) in Hiota.
             iEval (rewrite Hiota) in "Hcr".
-            iDestruct (lc_split (ι2 `min` ι3) (ι3 - (ι2 `min` ι3)) with "Hcr") as "[Hcr2 Hcr2']". iFrame.
+            iDestruct (lc_split (ι2 `min` ι3) (ι3 - (ι2 `min` ι3)) with "Hcr") as "[Hcr2 Hcr2']". setoid_rewrite trnsl_assertion_unfold. iFrame.
 
-        - iIntros (Φ). iModIntro. iIntros "[[Hstk Hu] Hcr] HΦ".
+        - iIntros (Φ). iModIntro. setoid_rewrite trnsl_assertion_unfold. iIntros "[[Hstk Hu] Hcr] HΦ".
           destruct b0.
-          + iApply (wp_if_t e (to_rtstmt stk_id s) (to_rtstmt stk_id s0) stk_id (symb_stk_to_stk_frm stk1 mp) (u ∗ £ι1) (stack_own[ stk_id, symb_stk_to_stk_frm stk2 mp] ∗ u0 ∗ £ι2) (lang.LitUnit) (inv_set_to_namespace mask) with "[IH'] [IH' Hstk Hu Hcr] [HΦ]"); try iFrame.
+          + iApply (wp_if_t e (to_rtstmt stk_id s) (to_rtstmt stk_id s0) stk_id (symb_stk_to_stk_frm stk1 mp) ((trnsl_assertion p stk_id mp) ∗ £ι1) (stack_own[ stk_id, symb_stk_to_stk_frm stk2 mp] ∗ (trnsl_assertion q stk_id mp) ∗ £ι2) (lang.LitUnit) (inv_set_to_namespace mask) with "[IH'] [IH' Hstk Hu Hcr] [HΦ]"); try iFrame.
             *  apply (trnsl_expr_interp_lexpr_compatibility _ e lexpr (LitBool true) mp); try done.
 
             * iIntros (Φ'). iModIntro. iIntros "[Hstk [Hu Hcr]] HΦ'".
+            setoid_rewrite trnsl_assertion_unfold.
             iPoseProof ("IH'" with "[%] [Hstk Hu Hcr]" ) as "HQ"; try done; try iFrame.
             { iPureIntro. unfold LExpr_holds. rewrite Hinterp_lexpr. done.  }
             iApply "HQ"; iFrame. iNext. iIntros "[[Hstk Hu] Hcr]". iApply "HΦ'". iFrame.
+
+            * setoid_rewrite trnsl_assertion_unfold. iFrame.
 
             * iNext. iIntros "[Hstk [Hu Hcr]]". iApply "HΦ". iFrame.
             assert (ι2 = ι2 `min` ι3 + (ι2 - ι2 `min` ι3)) as Hiota. { lia.  }
             apply (f_equal lc) in Hiota.
             iEval (rewrite Hiota) in "Hcr".
-            iDestruct (lc_split (ι2 `min` ι3) (ι2 - (ι2 `min` ι3)) with "Hcr") as "[Hcr2 Hcr2']". iFrame.
+            iDestruct (lc_split (ι2 `min` ι3) (ι2 - (ι2 `min` ι3)) with "Hcr") as "[Hcr2 Hcr2']". setoid_rewrite trnsl_assertion_unfold. iFrame.
             
-          + iApply (wp_if_f e (to_rtstmt stk_id s) (to_rtstmt stk_id s0) stk_id (symb_stk_to_stk_frm stk1 mp) (u ∗ £ι1) (stack_own[ stk_id, symb_stk_to_stk_frm stk2 mp] ∗ u0 ∗ £ι3) (lang.LitUnit) (inv_set_to_namespace mask) with "[IH'] [IH' Hstk Hu Hcr] [HΦ]"); try iFrame.
+          + iApply (wp_if_f e (to_rtstmt stk_id s) (to_rtstmt stk_id s0) stk_id (symb_stk_to_stk_frm stk1 mp) ((trnsl_assertion p stk_id mp) ∗ £ι1) (stack_own[ stk_id, symb_stk_to_stk_frm stk2 mp] ∗ (trnsl_assertion q stk_id mp) ∗ £ι3) (lang.LitUnit) (inv_set_to_namespace mask) with "[IH'] [IH' Hstk Hu Hcr] [HΦ]"); try iFrame.
             * apply (trnsl_expr_interp_lexpr_compatibility _ e lexpr (LitBool false) mp); try done.
 
             * iIntros (Φ'). iModIntro. iIntros "[Hstk [Hu Hcr]] HΦ'".
+            setoid_rewrite trnsl_assertion_unfold.
             iPoseProof ("IH1'" with "[%] [Hstk Hu Hcr]" ) as "HQ"; try done; try iFrame.
-            { iPureIntro. unfold LExpr_holds. simpl. rewrite Hinterp_lexpr. done.  }
+            { iPureIntro. unfold LExpr_holds. simpl. rewrite Hinterp_lexpr. done. }
             iApply "HQ"; iFrame. iNext. iIntros "[[Hstk Hu] Hcr]". iApply "HΦ'". iFrame.
+
+            * setoid_rewrite trnsl_assertion_unfold. iFrame.
 
             * iNext. iIntros "[Hstk [Hu Hcr]]". iApply "HΦ". iFrame.
 
             assert (ι3 = ι2 `min` ι3 + (ι3 - ι2 `min` ι3)) as Hiota. { lia.  }
             apply (f_equal lc) in Hiota.
             iEval (rewrite Hiota) in "Hcr".
-            iDestruct (lc_split (ι2 `min` ι3) (ι3 - (ι2 `min` ι3)) with "Hcr") as "[Hcr2 Hcr2']". iFrame.
+            iDestruct (lc_split (ι2 `min` ι3) (ι3 - (ι2 `min` ι3)) with "Hcr") as "[Hcr2 Hcr2']". setoid_rewrite trnsl_assertion_unfold. iFrame.
 
       }
       
@@ -918,14 +934,6 @@ Section MainTranslation.
         pose proof H0 as Hspec_StackFree.
         apply proc_spec_stack_free in Hspec_StackFree.
 
-        destruct (trnsl_assertion Γ (LAnd (LStack stk) (LAnd (LProc proc_name proc_record) (subst (proc_precond_of proc_record) subst_map))) stk_id mp) eqn:HPreCond; try done.
-
-        destruct (trnsl_assertion Γ
-          (LExists lvar_x
-          (LAnd (LStack (<[x:=lvar_x]> stk))
-          (subst (proc_postcond_of proc_record) (<["#ret_var":=LVar lvar_x]> subst_map)))) stk_id mp
-        ) eqn:HPostCond; try done.
-
         inversion Hwelldef; subst ρ0 v proc args0.
 
         assert (exists arg_vals, Forall2 (fun e v => expr_step e (symb_stk_to_stk_frm stk mp) (Val v)) args arg_vals) as Harg_vals.
@@ -933,7 +941,7 @@ Section MainTranslation.
         { 
           (* Prove existence of arg_vals *)
           clear Hwelldef H1 H4 H11.
-          clear subst_map HPreCond HPostCond.
+          clear subst_map.
           revert lexprs H2 H12. 
           induction args as [| a args IH]; intros lexprs H2 H12.
           - simpl in H2. destruct lexprs; [ | discriminate ]. exists nil. constructor.
@@ -958,7 +966,7 @@ Section MainTranslation.
 
         assert (Forall2 (λ expr val, interp_lexpr expr mp = Some (trnsl_val val)) lexprs arg_vals) as Hlexprs_arg_vals.
           {
-            clear Hwelldef H1  H4 H11 H12 subst_map HPreCond HPostCond.
+            clear Hwelldef H1  H4 H11 H12 subst_map.
             revert args arg_vals H2 Harg_vals.
             induction lexprs as [| le lexprs IH]; intros args arg_vals H2 Harg_vals.
             - destruct args; [| discriminate]. inversion Harg_vals. constructor.
@@ -974,39 +982,32 @@ Section MainTranslation.
 
         simpl in *.
         destruct proc_record as [proc_args proc_locals proc_pre proc_post proc_body] eqn:Hproc_record.
-        destruct (trnsl_stmt (proc_body)) eqn:Hproc_body, (trnsl_assertion Γ (subst proc_pre subst_map) stk_id mp) eqn:Hproc_pre; try rewrite Hproc_pre in HPreCond;  try discriminate; simpl in HPreCond.
+
+        set (trnsl_assertion (subst proc_pre subst_map) stk_id mp) as u1.
+
+        assert (trnsl_assertion (subst proc_pre subst_map) stk_id mp = u1) as Hproc_pre.
+            { subst u1; done. }
+
+        destruct (trnsl_stmt (proc_body)) eqn:Hproc_body;  try discriminate.
+
         
         {   
           (* proc_body = Skip *)
-        inversion H4; subst s. inversion HPreCond; subst u; clear HPreCond.
-        inversion HPostCond as [ HPostCond']; clear HPostCond.
-        iIntros (Φ). iModIntro.
+        inversion H4; subst s.
+        iIntros (Φ). iModIntro. setoid_rewrite trnsl_assertion_unfold.
         
         iIntros "[[Hstk [Hproc_tbl Hu1]] Hcr] HΦ".
 
-        pose proof (proc_specs_valid Γ proc_name (Proc proc_args proc_locals proc_pre proc_post proc_body) arg_vals ) as [ret_val Hproc]; try done.
+        pose proof (proc_specs_valid proc_name (Proc proc_args proc_locals proc_pre proc_post proc_body) arg_vals ) as [ret_val Hproc]; try done.
 
         set (subst_map' := @list_to_map var LExpr (gmap var LExpr) _ _ (zip (proc_args).*1 (map (λ val, LVal (trnsl_val val)) arg_vals))).
 
-          destruct (trnsl_assertion Γ (subst proc_pre subst_map') stk_id mp) as [ proc_frame_pre |] eqn: Hproc_frame_pre.
-          
-          2 : {  
-            (* trnsl_assertion (subst proc_pre subst_map') stk_id' mp CANNOT BE None *)
-            assert (is_Some (trnsl_assertion Γ (subst proc_pre subst_map') stk_id mp )) as Htrnsl_assertion. 
-            { apply trnsl_assertion_is_some. }
-            destruct Htrnsl_assertion as [v Htrnsl_assertion]. rewrite Htrnsl_assertion in Hproc_frame_pre. discriminate.
-          }
+          set ((trnsl_assertion (subst proc_pre subst_map') stk_id mp)) as proc_frame_pre.
+          set (trnsl_assertion (subst proc_post (<["#ret_val":=LVal (trnsl_val ret_val)]> subst_map')) stk_id mp) as proc_frame_post.
 
-          destruct (trnsl_assertion Γ (subst proc_post (<["#ret_val":=LVal (trnsl_val ret_val)]> subst_map')) stk_id mp) as [ proc_frame_post |] eqn: Hproc_frame_post.
 
-          2 : {
-            (* trnsl_assertion (subst proc_pre subst_map') stk_id' mp CANNOT BE None *)
-            assert (is_Some (trnsl_assertion Γ (subst proc_post
-                (<["#ret_val":=LVal (trnsl_val ret_val)]>
-              subst_map')) stk_id mp )) as Htrnsl_assertion. 
-            { apply trnsl_assertion_is_some. }
-            destruct Htrnsl_assertion as [v Htrnsl_assertion]. rewrite Htrnsl_assertion in Hproc_frame_post. discriminate.
-          }
+          assert ( trnsl_assertion (subst proc_post (<["#ret_val":=LVal (trnsl_val ret_val)]> subst_map')) stk_id mp = proc_frame_post) as Hproc_frame_post.
+          { subst proc_frame_post. done. }
 
         iApply (wp_call _ _ _ _ _ _ _ (lang.Proc proc_name proc_args proc_locals _) _ u1 proc_frame_post with "[] [Hstk Hproc_tbl Hu1]"); try iFrame; try done.
 
@@ -1030,9 +1031,12 @@ Section MainTranslation.
 
           simpl in HlocalsDef. pose proof (Hproc HlocalsDef) as Hproc.
 
-          rewrite (stack_free_assertion_trnsl Γ (subst proc_pre subst_map') stk_id stk_id' mp) in Hproc_frame_pre. 2 : { apply stack_free_assertion_subst. destruct Hspec_StackFree; done. }
+          assert (trnsl_assertion (subst proc_pre subst_map') stk_id mp = proc_frame_pre ) as Hproc_frame_pre.
+          { subst proc_frame_pre. done. }
 
-          rewrite (stack_free_assertion_trnsl Γ (subst proc_post (<["#ret_val":=LVal (trnsl_val ret_val)]> subst_map')) stk_id stk_id' mp) in Hproc_frame_post. 2 : { apply stack_free_assertion_subst. destruct Hspec_StackFree; done. }
+          rewrite (stack_free_assertion_trnsl (subst proc_pre subst_map') stk_id stk_id' mp) in Hproc_frame_pre. 2 : { apply stack_free_assertion_subst. destruct Hspec_StackFree; done. }
+
+          rewrite (stack_free_assertion_trnsl (subst proc_post (<["#ret_val":=LVal (trnsl_val ret_val)]> subst_map')) stk_id stk_id' mp) in Hproc_frame_post. 2 : { apply stack_free_assertion_subst. destruct Hspec_StackFree; done. }
 
           pose proof (Hproc Hproc_frame_pre Hproc_frame_post) as Hproc.
 
@@ -1046,15 +1050,18 @@ Section MainTranslation.
           iExists stk_frm''.
           
           iIntros (Φ'). iModIntro.
-          iIntros "[Hstk Hu1] HΦ".
+          iIntros "[Hstk Hu1] HΦ". 
+          instantiate (1 := lang.SkipS).
 
           iApply (Hproc with "[Hstk Hu1]").
 
           { 
-            rewrite (stack_free_assertion_trnsl Γ (subst proc_pre subst_map') stk_id' stk_id mp) in Hproc_frame_pre. 2 : { apply stack_free_assertion_subst. destruct Hspec_StackFree as [Hpre_stack_free _]. done. }
+            rewrite (stack_free_assertion_trnsl (subst proc_pre subst_map') stk_id' stk_id mp) in Hproc_frame_pre. 2 : { apply stack_free_assertion_subst. destruct Hspec_StackFree as [Hpre_stack_free _]. done. }
 
             iFrame.
-            pose proof (trnsl_assertion_w_lexpr_subst Γ proc_pre lexprs proc_args.*1 arg_vals stk_id mp u1 proc_frame_pre Hlexprs_arg_vals Hproc_pre Hproc_frame_pre) as Himpl.
+
+
+            pose proof (trnsl_assertion_w_lexpr_subst proc_pre lexprs proc_args.*1 arg_vals stk_id mp u1 proc_frame_pre Hlexprs_arg_vals Hproc_pre Hproc_frame_pre) as Himpl.
             iApply Himpl. iFrame.
           }
 
@@ -1062,63 +1069,52 @@ Section MainTranslation.
           iNext. iExact "HΦ".
           }
 
+          { rewrite Hproc_body. iFrame. setoid_rewrite <- trnsl_assertion_unfold. iFrame. }
+
           {
             iNext. iIntros "[Hstk [Hq Hcr']]".
             iApply "HΦ". iCombine "Hcr Hcr'" as "Hcr". rewrite Nat.add_1_r. iFrame. iExists (trnsl_val ret_val).
-          
-            destruct (trnsl_assertion Γ (subst proc_post (<["#ret_var":=LVar lvar_x]> subst_map)) stk_id
-            (λ x0 : lvar, if (x0 =? lvar_x)%string then trnsl_val ret_val else mp x0)) 
-            eqn:Hpost; try done.
+
+            set (trnsl_assertion (subst proc_post (<["#ret_var":=LVar lvar_x]> subst_map)) stk_id
+            (λ x0 : lvar, if (x0 =? lvar_x)%string then trnsl_val ret_val else mp x0)) as u.
+
+            assert ((trnsl_assertion (subst proc_post (<["#ret_var":=LVar lvar_x]> subst_map)) stk_id
+            (λ x0 : lvar, if (x0 =? lvar_x)%string then trnsl_val ret_val else mp x0)) = u) as Hpost.
+            { subst u; done. }
+
             
             iSplitR "Hq". 
             { rewrite fresh_mp_rewrite_symb_stk_to_stk_frm_compat; try done. rewrite trnsl_lval_trnsl_val_inverse. iFrame. } 
-            
-            { pose proof (trnsl_assertion_w_lexpr_subst_r Γ proc_post lexprs proc_args.*1 arg_vals lvar_x ret_val stk stk_id mp u proc_frame_post H Hlexprs_arg_vals Hpost Hproc_frame_post) as Himpl. iApply Himpl. iFrame. }
-            
-            
+
+            { pose proof (trnsl_assertion_w_lexpr_subst_r proc_post lexprs proc_args.*1 arg_vals lvar_x ret_val stk stk_id mp u proc_frame_post H Hlexprs_arg_vals Hpost Hproc_frame_post) as Himpl. 
+            setoid_rewrite <- trnsl_assertion_unfold. iApply Himpl. iFrame. }
           }
         }
 
         { (* proc body is not well-formed *)
 
-          inversion H4; subst s. inversion HPreCond; subst u; clear HPreCond. 
-          iIntros (Φ) "!> [[Hstk [Hfalse Hu]] Hcr]". done. 
+          inversion H4; subst s. 
+          setoid_rewrite trnsl_assertion_unfold.
+          iIntros (Φ) "!> [[Hstk [Hfalse Hu]] Hcr]". rewrite Hproc_body. done. 
         }
 
         {   
           (* proc_body != Skip *)
-        inversion H4; subst s. inversion HPreCond; subst u; clear HPreCond.
-        inversion HPostCond as [ HPostCond']; clear HPostCond.
+        inversion H4; subst s. 
         iIntros (Φ). iModIntro.
+        setoid_rewrite trnsl_assertion_unfold.
         
         iIntros "[[Hstk [Hproc_tbl Hu1]] Hcr] HΦ".
 
-        (* pose proof (proc_specs_valid proc_name (Proc proc_args proc_locals proc_pre proc_post proc_body) u1 u0 stk_id' mp lang.SkipS (inv_set_to_namespace mask) stk_frm' arg_vals) as [ret_val Hproc]. *)
-
-        (* destruct HPostCond' as [ret_val HPostCond]. *)
-
-        pose proof (proc_specs_valid Γ proc_name (Proc proc_args proc_locals proc_pre proc_post proc_body) arg_vals ) as [ret_val Hproc]; try done.
+        pose proof (proc_specs_valid proc_name (Proc proc_args proc_locals proc_pre proc_post proc_body) arg_vals ) as [ret_val Hproc]; try done.
 
         set (subst_map' := @list_to_map var LExpr (gmap var LExpr) _ _ (zip (proc_args).*1 (map (λ val, LVal (trnsl_val val)) arg_vals))).
 
-          destruct (trnsl_assertion Γ (subst proc_pre subst_map') stk_id mp) as [ proc_frame_pre |] eqn: Hproc_frame_pre.
-          
-          2 : {  
-            (* trnsl_assertion (subst proc_pre subst_map') stk_id' mp CANNOT BE None *)
-                        assert (is_Some (trnsl_assertion Γ (subst proc_pre subst_map') stk_id mp )) as Htrnsl_assertion. 
-            { apply trnsl_assertion_is_some. }
-            destruct Htrnsl_assertion as [v Htrnsl_assertion]. rewrite Htrnsl_assertion in Hproc_frame_pre. discriminate.
-          }
+          set (trnsl_assertion (subst proc_pre subst_map') stk_id mp) as proc_frame_pre.
+          assert ((trnsl_assertion (subst proc_pre subst_map') stk_id mp) = proc_frame_pre) as Hproc_frame_pre. { subst proc_frame_pre; done. }
 
-          destruct (trnsl_assertion Γ (subst proc_post (<["#ret_val":=LVal (trnsl_val ret_val)]> subst_map')) stk_id mp) as [ proc_frame_post |] eqn: Hproc_frame_post.
-
-          2 : {
-            (* trnsl_assertion (subst proc_pre subst_map') stk_id' mp CANNOT BE None *)
-            assert (is_Some (trnsl_assertion Γ (subst proc_post
-                (<["#ret_val":=LVal (trnsl_val ret_val)]> subst_map')) stk_id mp )) as Htrnsl_assertion. 
-            { apply trnsl_assertion_is_some. }
-            destruct Htrnsl_assertion as [v Htrnsl_assertion]. rewrite Htrnsl_assertion in Hproc_frame_post. discriminate.
-          }
+          set (trnsl_assertion (subst proc_post (<["#ret_val":=LVal (trnsl_val ret_val)]> subst_map')) stk_id mp) as proc_frame_post.
+          assert ((trnsl_assertion (subst proc_post (<["#ret_val":=LVal (trnsl_val ret_val)]> subst_map')) stk_id mp) = proc_frame_post) as Hproc_frame_post. { subst proc_frame_post; done. }
 
         iApply (wp_call _ _ _ _ _ _ _ (lang.Proc proc_name proc_args proc_locals _) _ u1 proc_frame_post with "[] [Hstk Hproc_tbl Hu1]"); try iFrame; try done.
 
@@ -1142,9 +1138,9 @@ Section MainTranslation.
 
           simpl in HlocalsDef. pose proof (Hproc HlocalsDef) as Hproc.
 
-          rewrite (stack_free_assertion_trnsl Γ (subst proc_pre subst_map') stk_id stk_id' mp) in Hproc_frame_pre. 2 : { apply stack_free_assertion_subst. destruct Hspec_StackFree; done. }
+          rewrite (stack_free_assertion_trnsl (subst proc_pre subst_map') stk_id stk_id' mp) in Hproc_frame_pre. 2 : { apply stack_free_assertion_subst. destruct Hspec_StackFree; done. }
 
-          rewrite (stack_free_assertion_trnsl Γ (subst proc_post (<["#ret_val":=LVal (trnsl_val ret_val)]> subst_map')) stk_id stk_id' mp) in Hproc_frame_post. 2 : { apply stack_free_assertion_subst. destruct Hspec_StackFree; done. }
+          rewrite (stack_free_assertion_trnsl (subst proc_post (<["#ret_val":=LVal (trnsl_val ret_val)]> subst_map')) stk_id stk_id' mp) in Hproc_frame_post. 2 : { apply stack_free_assertion_subst. destruct Hspec_StackFree; done. }
 
           pose proof (Hproc Hproc_frame_pre Hproc_frame_post) as Hproc.
 
@@ -1163,11 +1159,11 @@ Section MainTranslation.
           iApply (Hproc with "[Hstk Hu1]").
 
           { 
-            rewrite (stack_free_assertion_trnsl Γ (subst proc_pre subst_map') stk_id' stk_id mp) in Hproc_frame_pre. 2 : { apply stack_free_assertion_subst. destruct Hspec_StackFree as [Hpre_stack_free _]. done. }
+            rewrite (stack_free_assertion_trnsl (subst proc_pre subst_map') stk_id' stk_id mp) in Hproc_frame_pre. 2 : { apply stack_free_assertion_subst. destruct Hspec_StackFree as [Hpre_stack_free _]. done. }
 
 
             iFrame.
-            pose proof (trnsl_assertion_w_lexpr_subst Γ proc_pre lexprs proc_args.*1 arg_vals stk_id mp u1 proc_frame_pre Hlexprs_arg_vals Hproc_pre Hproc_frame_pre) as Himpl.
+            pose proof (trnsl_assertion_w_lexpr_subst proc_pre lexprs proc_args.*1 arg_vals stk_id mp u1 proc_frame_pre Hlexprs_arg_vals Hproc_pre Hproc_frame_pre) as Himpl.
             iApply Himpl. iFrame.
           }
 
@@ -1176,18 +1172,22 @@ Section MainTranslation.
 
           }
 
+          { rewrite Hproc_body. iFrame. setoid_rewrite <- trnsl_assertion_unfold. iFrame. }
+
           {
             iNext. iIntros "[Hstk [Hq Hcr']]".
             iApply "HΦ". iCombine "Hcr" "Hcr'" as "Hcr". rewrite Nat.add_1_r. iFrame. iExists (trnsl_val ret_val).
-          
-            destruct (trnsl_assertion Γ (subst proc_post (<["#ret_var":=LVar lvar_x]> subst_map)) stk_id
-            (λ x0 : lvar, if (x0 =? lvar_x)%string then trnsl_val ret_val else mp x0)) 
-            eqn:Hpost; try done.
+
+            set (trnsl_assertion (subst proc_post (<["#ret_var":=LVar lvar_x]> subst_map)) stk_id
+            (λ x0 : lvar, if (x0 =? lvar_x)%string then trnsl_val ret_val else mp x0)) as u.
+            assert ((trnsl_assertion (subst proc_post (<["#ret_var":=LVar lvar_x]> subst_map)) stk_id
+            (λ x0 : lvar, if (x0 =? lvar_x)%string then trnsl_val ret_val else mp x0)) = u) as Hpost. {subst u; done. }
             
             iSplitR "Hq". 
             { rewrite fresh_mp_rewrite_symb_stk_to_stk_frm_compat; try done. rewrite trnsl_lval_trnsl_val_inverse. iFrame. } 
             
-            { pose proof (trnsl_assertion_w_lexpr_subst_r Γ proc_post lexprs proc_args.*1 arg_vals lvar_x ret_val stk stk_id mp u proc_frame_post H Hlexprs_arg_vals Hpost Hproc_frame_post) as Himpl. iApply Himpl. iFrame. }
+            { pose proof (trnsl_assertion_w_lexpr_subst_r proc_post lexprs proc_args.*1 arg_vals lvar_x ret_val stk stk_id mp u proc_frame_post H Hlexprs_arg_vals Hpost Hproc_frame_post) as Himpl. 
+            setoid_rewrite <- trnsl_assertion_unfold. iApply Himpl. iFrame. }
           }
 
         }
@@ -1197,10 +1197,11 @@ Section MainTranslation.
       1 : {
         (* FPU *)
         unfold trnsl_hoare_triple; simpl.
+        setoid_rewrite trnsl_assertion_unfold.
         specialize (RAPack_fpuValid Γ RAPack old_val new_val) as HRA_fpu.
-        destruct (Γ RAPack) as [i [U [Hdisc [Heq_car [Hindx [Hcomp Hval]]]]]].
-
+        
         iIntros "[[Hstack Hown] Hcr]".
+        destruct (Γ RAPack) as [i [U [Hdisc [Heq_car [Hindx [Hcomp Hval]]]]]] eqn:H_RA_Pack.
         iDestruct "Hown" as (l) "[%Heq Hown]".
 
         iFrame.
@@ -1214,10 +1215,10 @@ Section MainTranslation.
 
        { apply transport_cmra_update. exact H0.  }
 
-       iModIntro. iExists l. iFrame. iPureIntro. exact Heq.
+       iModIntro. rewrite H_RA_Pack. iExists l. iFrame. iPureIntro. exact Heq.
 
       }
-      
+
     Qed.
   
   End MainTranslation.
